MathematicalLogic/FirstOrder/Completeness/TermModel.lean
@@ -1,0 +1,95 @@
+import MathematicalLogic.FirstOrder.Semantics
+import MathematicalLogic.FirstOrder.Completeness.Basic
+
+def Terms.ofVector : Vector (Term 𝓛) n → Terms 𝓛 n
+| ⟨l, h⟩ =>
+  match n, l with
+  | 0, [] => []ₜ
+  | n + 1, t :: l => t ∷ₜ Terms.ofVector ⟨l, by simp at h; exact h⟩
+
+@[simp] lemma Terms.of_vector_nil : Terms.ofVector Vector.nil = ([]ₜ : Terms 𝓛 0) := rfl
+@[simp] lemma Terms.of_vector_cons : Terms.ofVector (Vector.cons t v) = t ∷ₜ Terms.ofVector v := rfl
+
+instance : Coe (Vector (Term 𝓛) n) (Terms 𝓛 n) where
+  coe := Terms.ofVector
+
+@[reducible] def TermModel (Γ : Context 𝓛) : Model 𝓛 where
+  𝓤 := Term 𝓛
+  𝓕 := λ f ts => f ⬝ₜ ts
+  𝓟 := λ p ts => Γ ⊢ p ⬝ₚ ts
+
+local notation "𝓜ᵀ" => TermModel
+
+mutual
+theorem Term.interp_term_model :
+  ⟦ t ⟧ₜ 𝓜ᵀ Γ, ρ = t[ρ]ₜ :=
+  match t with
+  | #x => by simp [Term.interp]
+  | f ⬝ₜ ts => by simp [Term.interp]; rw [Terms.interp_term_model]
+theorem Terms.interp_term_model :
+  (⟦ ts ⟧ₜₛ 𝓜ᵀ Γ, ρ : Terms 𝓛 n) = ts[ρ]ₜₛ :=
+  match ts with
+  | []ₜ => by simp [Terms.interp]
+  | t ∷ₜ ts => by
+    simp [Terms.interp]
+    rw [Term.interp_term_model, Terms.interp_term_model]
+    trivial
+end
+termination_by
+  Term.interp_term_model => t.size
+  Terms.interp_term_model => ts.size
+
+lemma subst_const {c : Const 𝓛} : (c : Term 𝓛)[σ]ₜ = c := rfl
+
+lemma assignment_cons_in_term_model
+  {Γ : Context 𝓛} {ρ : Assignment (TermModel Γ)} :
+  ⇑ₛρ ∘ₛ ↦ₛ t = Assignment.cons (𝓜 := TermModel Γ) t ρ := by
+  funext x
+  cases x with
+  | zero => rfl
+  | succ x => simp [Subst.comp, Subst.lift, Term.shift_subst_single, Assignment.cons]
+
+theorem Formula.interp_term_model :
+  MaximalConsistent Γ → WitnessProperty Γ →
+  (⟦ p ⟧ₚ 𝓜ᵀ Γ, ρ ↔ Γ ⊢ p[ρ]ₚ) := by
+  rintro ⟨h₁, h₂⟩ h₃
+  induction p generalizing ρ <;> simp [Formula.interp]
+  case atom p ts => simp [Terms.interp_term_model]
+  case false => exact h₁
+  case implies p q ih₁ ih₂ =>
+    rw [ih₁, ih₂]
+    constructor
+    · intro h
+      rcases h₂ (p[ρ]ₚ) with h' | h'
+      · exact Proof.mp (Proof.axioms Axioms.a1) (h h')
+      · exact Proof.mp Proof.contradiction h'
+    · exact Proof.mp
+  case all p ih =>
+    constructor
+    · intro h₁'
+      rcases h₂ (∀' p[⇑ₛρ]ₚ) with h₂' | h₂'
+      · exact h₂'
+      · exfalso
+        apply Proof.mp Proof.not_forall at h₂'
+        apply h₃ at h₂'
+        rcases h₂' with ⟨c, h₂'⟩
+        simp [Formula.subst, Formula.subst_comp] at h₂'
+        rw [←subst_const (σ := ρ)] at h₂'
+        apply h₁
+        apply Proof.mp h₂'
+        rw [←ih, assignment_cons_in_term_model]
+        apply h₁'
+    · intros h t
+      apply Proof.mp (Proof.axioms (Axioms.a4 (t := t))) at h
+      rw [Formula.subst_comp, ←ih, assignment_cons_in_term_model] at h
+      exact h
+
+theorem satisfiable_by_term_model :
+  MaximalConsistent Γ → WitnessProperty Γ → Satisfiable Γ := by
+  intros h₁ h₂
+  apply Satisfiable.up.{0}
+  exists 𝓜ᵀ Γ, Subst.id
+  intros p h
+  rw [Formula.interp_term_model h₁ h₂, Formula.subst_id]
+  apply Proof.assumption
+  exact h
